\question

\begin{parts}

\part[5] % RS 6A, Q1c).
Prove Theorem~\ref{thm:sum-of-geometric-sequence} by mathematical induction.

\begin{EnvFullwidth}
\begin{solutionorgrid}[4.5in]
\begin{proof}
$P(n)$ is: $\displaystyle{\sum_{j = 0}^{n - 1} r^j = \frac{r^n - 1}{r - 1}}$, for all $n \in \Z^+$.

\textbf{Basis}: If $n = 1$, the LHS is $r^{1 - 1} = r^0 = 1$ and the RHS is $\displaystyle{\frac{r^1 - 1}{r - 1}} = 1$. So $P(1)$ is true.

\textbf{Inductive step}: If $P(k)$ is true then $\displaystyle{\sum_{j = 0}^{k - 1} r^j = \frac{r^k - 1}{r - 1}}$, for all $k \in \Z^+$. Now,
\begin{align*}
    \sum_{j = 0}^k r^j &= \frac{r^k - 1}{r - 1} + r^{k} && (\textrm{by hypothesis}) \\
    &= \frac{r^k - 1}{r - 1} + \frac{r^{k}(r - 1)}{(r - 1)} \\
    &= \frac{r^k - 1 + r^{k + 1} - r^k}{r - 1} \\
    &= \frac{r^{k + 1} - 1}{r - 1}.
\end{align*}
Since $P(1)$ is true and $P(k) \implies P(k + 1)$, by the PMI, $P(n)$ is true for all $n \in \Z^+$.
\end{proof}
\end{solutionorgrid}
\end{EnvFullwidth}

\part[2]
Hence, find $\displaystyle{1 + \frac{1}{2} + \frac{1}{4} + \frac{1}{8} + \cdots + \frac{1}{256} = \sum_{j = 0}^{8} \pfrac{1}{2}^{\! j}.}$ in the form $\displaystyle{\frac{m}{n}}$.

\begin{EnvFullwidth}
\begin{solutionorgrid}[2.5in]
By Theorem~\ref{thm:sum-of-geometric-sequence}, on putting $r = \frac{1}{2}$ and $n - 1 = 8$ we get
\begin{align*}
    \sum_{j = 0}^{8} \pfrac{1}{2}^{\! j} &= \frac{(\frac{1}{2})^9 - 1}{\frac{1}{2} - 1} \\
    &= \frac{\frac{1}{512} - \frac{512}{512}}{-\frac{1}{2}} \\
    &= \frac{-\frac{511}{512}}{-\frac{1}{2}} \\
    &= \frac{511}{256}.
\end{align*}
\end{solutionorgrid}
\end{EnvFullwidth}

\end{parts}
