\question % Ex. 3L, Q7.
Consider isosceles triangle $OAB$ shown in Figure~\ref{fig:bisector-is-perpendicular}. Let $\vv{OA} = \vec{a}$ and $\vv{OB} = \vec{b}$.

\begin{figure}[h]
    \centering
    \begin{tikzpicture}
    \tkzDefPoint(0,0){O}
    \tkzDefShiftPoint[O](240:4.5){A}
    \tkzDefShiftPoint[O](300:4.5){B}
    \tkzDefMidPoint(A,B)
    \tkzGetPoint{M}
    \tkzLabelPoint[right](O){$O$}
    \tkzLabelPoint[left](A){$A$}
    \tkzLabelPoint[right](B){$B$}
    \tkzLabelPoint[below](M){$M$}
    \ifprintanswers
    \tkzDrawSegments[vector,color=red](O,A O,B O,M A,B)
    \tkzMarkSegment[mark=|,color=red](O,A)
    \tkzMarkSegment[mark=|,color=red](O,B)
    \tkzMarkSegment[mark=||,color=red](A,M)
    \tkzMarkSegment[mark=||,color=red](B,M)
    \tkzLabelSegment[pos=.6,left,color=red](O,A){$\vec{a}$}
    \tkzLabelSegment[pos=.6,right,color=red](O,B){$\vec{b}$}
    \tkzLabelSegment[pos=.6,left,color=red](O,M){$\vv{OM}$}
    \else
    \tkzMarkSegment[mark=|](O,A)
    \tkzMarkSegment[mark=|](O,B)
    \tkzMarkSegment[mark=||](A,M)
    \tkzMarkSegment[mark=||](B,M)
    \tkzDrawPolygon[semithick](O,A,B)
    \tkzDrawPoint(M)
    \fi
    \end{tikzpicture}
    \caption{Isosceles triangle $ABC$.}
    \label{fig:bisector-is-perpendicular}
\end{figure}

\begin{parts}

\part[1]
Draw vector $\vv{OM}$ on Figure~\ref{fig:bisector-is-perpendicular}.

\part[2]
Find $\vv{AB}$ and $\vv{OM}$ in terms of $\vec{a}$ and $\vec{b}$.

\begin{EnvFullwidth}
\begin{solutionorgrid}[2in]
We have
\[
    \vv{AB} = \vec{b} - \vec{a},
\]
and
\[
    \vv{OM} = \vv{OA} + \frac{1}{2}\vv{AB} = \vec{a} + \frac{1}{2}(\vec{b} - \vec{a}) = \frac{1}{2}(\vec{b} + \vec{a}).
\]
\end{solutionorgrid}
\end{EnvFullwidth}

\part[3]
Hence, use vectors to prove Proposition~\ref{prop:bisector-is-perpendicular}.

\begin{EnvFullwidth}
\begin{solutionorgrid}[2.5in]
\begin{proof}
We have
\begin{align*}
    \vv{OM} \cdot \vv{AB} &= \frac{1}{2}(\vec{b} + \vec{a}) \cdot (\vec{b} - \vec{a}) && (\textrm{by (b)}) \\
    &= \frac{1}{2}(\vec{b} \cdot \vec{b} \cancel{- \vec{b} \cdot \vec{a} + \vec{a} \cdot \vec{b}} - \vec{a} \cdot \vec{a}) \\
    &= \abs{\vec{b}}^2 - \abs{\vec{a}}^2 \\
    &= 0 && (\triangle OAB \textrm{ is isosceles}).
\end{align*}
A zero dot product implies perpendicularity.
\end{proof}
\end{solutionorgrid}
\end{EnvFullwidth}

\end{parts}
