\question[4]
Prove Theorem~\ref{thm:difference-of-sine-squares}.

\begin{EnvFullwidth}
\begin{solutionorgrid}[5in]
\begin{proof}
Let $A = \sin(\theta + \varphi)$ and $B = \sin(\theta - \varphi)$. By the angle sum identities
\[
	A = \sin(\theta)\cos(\varphi) + \sin(\varphi)\cos(\theta),
\]
and
\[
	B = \sin(\theta)\cos(\varphi) - \sin(\varphi)\cos(\theta).
\]
Thus
\begin{align*}
	AB &= (\sin(\theta)\cos(\varphi) + \sin(\varphi)\cos(\theta)) \times (\sin(\theta)\cos(\varphi) - \sin(\varphi)\cos(\theta)) \\
	&= (\sin(\theta)\cos(\varphi))^2 - \sin(\theta)\sin(\varphi)\cos(\theta)\cos(\varphi) + \sin(\theta)\sin(\varphi)\cos(\theta)\cos(\varphi) - (\sin(\varphi)\cos(\theta))^2 \\
	&= \sin^2(\theta)\cos^2(\varphi) - \sin^2(\varphi)\cos^2(\theta) \\
	&= \sin^2(\theta)(1 - \sin^2(\varphi)) - \sin^2(\varphi)(1 - \sin^2(\theta)) \\
	&= \sin^2(\theta) - \sin^2(\theta)\sin^2(\varphi) - \sin^2(\varphi) + \sin^2(\theta)\sin^2(\varphi) \\
	&= \sin^2(\theta) - \sin^2(\varphi).
\end{align*}
\end{proof}
\end{solutionorgrid}
\end{EnvFullwidth}
