\question[4]
Use Theorem~\ref{thm:sum-to-product-identities-for-sine} to find $\sin(3\theta) - \sin(\theta)$ and hence, prove Theorem~\ref{thm:triple-angle-formula-for-sine}.

\begin{EnvFullwidth}
\begin{solutionorgrid}[4.5in]
\begin{proof}
We have
\begin{align*}
	\sin(3\theta) - \sin(\theta) &= 2\cos\! \left( \frac{3\theta + \theta}{2} \right) \sin\! \left( \frac{3\theta - \theta}{2} \right) && (\textrm{By Theorem~\ref{thm:sum-to-product-identities-for-sine}}) \\
	&= 2\cos(2\theta)\sin(\theta) \\
	&= 2\sin(\theta)(1 - 2\sin^2(\theta)) \\
	&= 2\sin(\theta) - 4\sin^3(\theta).
\end{align*}
Thus, $\sin(3\theta) = 3\sin(\theta) - 4\sin^3(\theta)$.
\end{proof}
\end{solutionorgrid}
\end{EnvFullwidth}
